thys/MSO_Regex_Equivalence/Pi_Regular_Exp_Dual.thy
@@ -17,7 +17,7 @@ datatype_new 'a rexp_dual =
   CoTimes (co: bool) "'a rexp_dual" "'a rexp_dual" |
   CoStar (co: bool) "'a rexp_dual" |
   CoPr (co: bool) "'a rexp_dual"
-datatype_new_compat rexp_dual
+datatype_compat rexp_dual
 derive linorder rexp_dual
 
 abbreviation "CoPLUS_dual b \<equiv> rexp_of_list (CoPlus b) (CoZero b)"
@@ -215,7 +215,7 @@ next
   case "5_9" thus ?case by auto
 next
   case "5_10" thus ?case
-    by auto (metis (no_types, hide_lams) Cons_in_lists_iff Diff_iff imageI map.simps lists.Nil)+
+    by auto (metis (no_types, hide_lams) Cons_in_lists_iff Diff_iff imageI list.simps(8) list.simps(9) lists.Nil)+
 next
   case "5_11" thus ?case by auto
 next
@@ -241,7 +241,7 @@ next
   case "5_21" thus ?case by auto
 next
   case "5_22" thus ?case
-    by auto (metis (no_types, hide_lams) Cons_in_lists_iff Diff_iff imageI map.simps lists.Nil)+
+    by auto (metis (no_types, hide_lams) Cons_in_lists_iff Diff_iff imageI list.simps(8) list.simps(9) lists.Nil)+
 next
   case "5_23" thus ?case by auto
 next
